slice_u8_eq_ascii_string

src/cddl/pulse/CDDL.Pulse.Misc.fst
@@ -5,6 +5,7 @@ open Pulse.Lib.Pervasives
 module Trade = Pulse.Lib.Trade.Util
 open CBOR.Spec.API.Type
 open CBOR.Pulse.API.Base
+module AST = CDDL.Spec.AST.Base
 
 inline_for_extraction noextract [@@noextract_to "krml"]
 ```pulse
@@ -138,3 +139,136 @@ fn impl_str_size
     }
 }
 ```
+
+module U8 = FStar.UInt8
+
+inline_for_extraction noextract
+let slice_u8_eq_list_ascii_char_t
+  (l: list FStar.Char.char)
+: Tot Type
+= (s: S.slice U8.t) ->
+  (i: SZ.t) ->
+  (#p: perm) ->
+  (#v: Ghost.erased (Seq.seq U8.t)) ->
+  stt bool
+    (pts_to s #p v **
+      pure (
+        SZ.v i + List.Tot.length l <= Seq.length v /\
+True //        List.Tot.for_all AST.char_is_ascii l
+      )
+    )
+    (fun res ->
+      pts_to s #p v **
+      pure (
+        SZ.v i + List.Tot.length l <= Seq.length v /\
+True /\ //        List.Tot.for_all AST.char_is_ascii l /\
+        (res == true <==> Seq.equal
+          (Seq.slice v (SZ.v i) (SZ.v i + List.Tot.length l))
+          (Seq.seq_of_list (AST.byte_list_of_char_list l))
+        )
+      )
+    )
+
+inline_for_extraction
+```pulse
+fn slice_u8_eq_list_ascii_char_nil (_: unit) : slice_u8_eq_list_ascii_char_t []
+= (s: _)
+  (i: _)
+  (#p: _)
+  (#v: _)
+  {
+    true
+  }
+```
+
+let list_map_cons
+  (#t #t': Type)
+  (f: t -> t')
+  (a: t)
+  (q: list t)
+: Lemma
+  (List.Tot.map f (a :: q) == f a :: List.Tot.map f q)
+= ()
+
+module U32 = FStar.UInt32
+
+inline_for_extraction
+```pulse
+fn slice_u8_eq_list_ascii_char_cons (a: FStar.Char.char) (a' : U8.t) (sq: squash (a' == AST.uint32_to_uint8 (AST.u32_of_char a) /\ AST.char_is_ascii a)) (q: list FStar.Char.char) (f: slice_u8_eq_list_ascii_char_t q) : slice_u8_eq_list_ascii_char_t (a :: q)
+= (s: _)
+  (i: _)
+  (#p: _)
+  (#v: _)
+  {
+    S.pts_to_len s;
+    FStar.Math.Lemmas.small_mod (FStar.UInt32.v (AST.u32_of_char a)) 256;
+    Seq.lemma_seq_of_list_cons (a' <: U8.t) (AST.byte_list_of_char_list q);
+    list_map_cons AST.u32_of_char a q;
+    list_map_cons AST.uint32_to_uint8 (AST.u32_of_char a) (List.Tot.map AST.u32_of_char q);
+    assert (pure (AST.byte_list_of_char_list (a :: q) == AST.uint32_to_uint8 (AST.u32_of_char a) :: AST.byte_list_of_char_list q));
+    assert (pure (AST.byte_list_of_char_list (a :: q) == a' :: AST.byte_list_of_char_list q));
+    assert (pure (Seq.equal (Seq.seq_of_list (AST.byte_list_of_char_list (a :: q))) (Seq.cons a' (Seq.seq_of_list (AST.byte_list_of_char_list q)))));
+    let x = S.op_Array_Access s i;
+    let i' = SZ.add i 1sz;
+    assert (pure (Seq.equal (Seq.slice v (SZ.v i) (SZ.v i + List.Tot.length (a :: q))) (Seq.cons x (Seq.slice v (SZ.v i') (SZ.v i' + List.Tot.length q)))));
+    Classical.move_requires (Seq.lemma_cons_inj x a' (Seq.slice v (SZ.v i') (SZ.v i' + List.Tot.length q))) (Seq.seq_of_list (AST.byte_list_of_char_list q));
+    if (x = a') {
+      f s i'
+    } else {
+      false
+    }
+  }
+```
+
+let rec slice_u8_eq_list_ascii_char
+  (l: list FStar.Char.char)
+  (sq: squash (List.Tot.for_all AST.char_is_ascii l))
+: Tot (slice_u8_eq_list_ascii_char_t l)
+= match l with
+  | [] -> slice_u8_eq_list_ascii_char_nil ()
+  | a :: q -> slice_u8_eq_list_ascii_char_cons a (AST.uint32_to_uint8 (AST.u32_of_char a)) () q (slice_u8_eq_list_ascii_char q ())
+
+inline_for_extraction noextract
+let slice_u8_eq_ascii_string_t
+  (x: AST.ascii_string)
+: Tot Type
+= (s: S.slice U8.t) ->
+  (i: SZ.t) ->
+  (#p: perm) ->
+  (#v: Ghost.erased (Seq.seq U8.t)) ->
+  stt bool
+    (pts_to s #p v **
+      pure (
+        SZ.v i + FStar.String.length x <= Seq.length v
+      )
+    )
+    (fun res ->
+      pts_to s #p v **
+      pure (
+        SZ.v i + FStar.String.length x <= Seq.length v /\
+        (res == true <==> Seq.equal
+          (Seq.slice v (SZ.v i) (SZ.v i + FStar.String.length x))
+          (AST.byte_seq_of_ascii_string x)
+        )
+      )
+    )
+
+inline_for_extraction noextract
+```pulse
+fn slice_u8_eq_ascii_string_intro
+  (x: AST.ascii_string)
+  (f: slice_u8_eq_list_ascii_char_t (FStar.String.list_of_string x))
+: slice_u8_eq_ascii_string_t x
+= (s: S.slice U8.t)
+  (i: SZ.t)
+  (#p: perm)
+  (#v: Ghost.erased (Seq.seq U8.t))
+{
+  f s i
+}
+```
+
+let slice_u8_eq_ascii_string
+  (x: AST.ascii_string)
+: Tot (slice_u8_eq_ascii_string_t x)
+= slice_u8_eq_ascii_string_intro x (slice_u8_eq_list_ascii_char (FStar.String.list_of_string x) ())
